---
tags:
  - Maths
date: 2025-01-16
title: Roots of polynomials
---
---  
# Greek alphabet  
$\alpha$ alpha  
$\beta$ beta  
$\gamma$ gamma  
$\delta$ delta  
  
# Roots of polynomials  
## Quadratic  
$ax^2+bx+c=0 \rightarrow x^2+\frac{b}{a}{x}+\frac{c}{a}=0$  
roots of $x=\alpha\space{or}\space{x}=\beta$  
$(x-\alpha)(x-\beta)=0$  
$x^2-\alpha{x}-\beta{x}+\alpha\beta$  
$x^2-(\beta+\alpha)x+\alpha\beta$  
  
## Cubic  
$ax^3+bx^2+cx+d=0 \rightarrow x^3+\frac{b}{a}x^2+\frac{c}{a}x+\frac{d}{a}=0$  
3 roots  
$(x-\alpha)(x-\beta)(x-\gamma)=0$  
$(x^2-\alpha{x}-\beta{x}+\alpha\beta)(x-\gamma)=0$  
$(x^3-\alpha{x^2}-\beta{x^2}+\alpha\beta{x}-\gamma{x^2}+\alpha\gamma{x}+\beta\gamma{x}-\alpha\beta\gamma)=0$  
$(\alpha+\beta+\gamma)=\frac{-b}{a}$  
$(\alpha\beta+\alpha\gamma+\beta\gamma)=\frac{c}{a}$  
$(\alpha\beta\gamma)=\frac{-d}{a}$  
  
## Quartic  
$ax^4+bx^3+cx^2+dx+e \rightarrow x^4+\frac{b}{a}x^3+\frac{c}{a}x^2+\frac{d}{a}x+\frac{e}{a}$  
$(x-\alpha)(x-\beta)(x-\gamma)(x-\delta)=0$  
$x^4-(\alpha+\beta+\gamma+\delta)x^3+(\alpha\beta+\alpha\gamma+\alpha\delta+\beta\gamma+\beta\delta+\gamma\delta)x^2-(\alpha\beta\gamma+\alpha\beta\delta+\alpha\gamma\delta+\beta\gamma\delta)x+(\alpha\beta\gamma\delta)=0$  
  
$(\alpha+\beta+\gamma+\delta)=\frac{-b}{a}$  
$(\alpha\beta+\alpha\gamma+\alpha\delta+\beta\gamma+\beta\delta+\gamma\delta)=\frac{c}{a}$  
$(\alpha\beta\gamma+\alpha\beta\delta+\alpha\gamma\delta+\beta\gamma\delta)=\frac{-d}{a}$  
$(\alpha\beta\gamma\delta)=\frac{e}{a}$  
  
Shorthand= $x^4-\sum\alpha x^3+\sum\alpha\beta x^2-\sum\alpha\beta\gamma x+\sum\alpha\beta\gamma\delta=0$  
  
## Example  
a) $\alpha+\beta=\frac{-b}{a}$  
$\alpha+\beta=7\qquad\alpha\beta=12$  
b) $\alpha^2+\beta^2=25\qquad(\alpha+\beta)^2=\alpha^2+2\alpha\beta+\beta^2$  
$49=\alpha^2+\beta^2+2\alpha\beta\qquad49=\alpha^2+\beta^2+2(12)$  
$25=\frac{-b}{a}\qquad144=\frac{c}{a}$  
$\alpha^2\beta^2=144\qquad{x}^2-25x+144=0$  
  
## Example 2  
$\frac{1}{\alpha}+\frac{1}{\beta}=\frac{\alpha+\beta}{\alpha\beta}=\frac{7}{12}=\frac{-b}{a} \Rightarrow a=12\quad{b}=-7\quad{c}=1$  
  
## Question 1  
a) $x^2-5x+9=0\qquad{x}^2-\sum{\alpha}x+\sum{\alpha\beta}\qquad(\alpha+\beta)=-(-5) \Rightarrow \alpha+\beta=5$  
  
