---
tags:
  - Maths
  - Pure
date: 2025-01-23
---
---  
# Starter  
$x^2-4x-6y+y^2=12$  
$x^2-4x=12 \qquad (x-2)^2 - 2^2 - 12 = 0 \qquad (x-2)^2 - 16 =0 \qquad (x-2)^2 = 16 \qquad x-2=\pm \sqrt{16} \qquad x=\pm 4 + 2$   
for positive x value, $x = 4+2 = 6$  
  
$x^2-4x=(x-2)^2-4$  
$y^2-6y=(y-3)^2-9$  
$(x-2)^2-4+(y-3)^2-9=12$  
$(x-2)^2+(y-2)^2=25$  
center is $(2,3)$  
grad of normal is $\frac{3}{4}$  
grad of tangent is $-\frac{4}{3}$  
$y=-\frac{4}{3}x+c$  
sub in $(6,0)$  
$0=-8+c \qquad c=8$  
eq of tangent is $y=-\frac{4}{3}x+8$  
  
# [[./index|Roots of polynomials]]  
The roots of $x^2-7x+12$ are $x=\alpha$ and $x=\beta$  
a. $\alpha + \beta = 7 \qquad \alpha \beta = 12$  
b. $(\alpha + \beta)^2 = \alpha ^2 + \beta ^2 + 2(\alpha \beta)$  
$49= \alpha ^2 + \beta ^2 + 2(12)$  
$\alpha ^2 + \beta ^2 = 49-24 =25 = \frac{-b}{a}$  
$\alpha ^2 \beta ^2 = (\alpha \beta)^2 = 12^2 = 144 = \frac{c}{a}$  
$a=1 \qquad b=-25 \qquad c=144$  
$x^2-25x+144=0$  
$\frac{1}{\alpha} + \frac{1}{\beta} = \frac{\alpha + \beta}{\alpha \beta} = \frac{7}{12} = \frac{-b}{a}$  
$\frac{1}{\alpha} \times \frac{1}{\beta} = \frac{1}{\alpha \beta} = \frac{1}{12} = \frac{c}{a}$  
$a=12 \qquad b=-7 \qquad c=1$  
$12x^2-7x+1$  
  
## Practise  
4. $p(x)=0$  
$\sum \alpha = \frac{-b}{a} = 5 \qquad \therefore b=-5$  
$\sum \alpha \beta = \frac{c}{a} = 4 \qquad \therefore c=4$  
$\sum \alpha \beta \gamma = \frac{-d}{a} - 2 \qquad \therefore d=2$  
$x^3-5x^2+4x+2=0$  
  
5.   
	1. $x^4-13x^2+36=0$  
		1. $\sum \alpha = 0$  
		$\sum \alpha \beta = -13$  
		$\sum \alpha \beta \gamma = 0$  
		$\sum \alpha \beta \gamma \delta = 36$  
		$(\alpha + \beta + \gamma + \delta)^2 - 2(\sum \alpha \beta) = \alpha^2 + \beta^2 + \gamma^2 +\delta^2$  
		$\therefore \alpha^2 + \beta^2 + \gamma^2 +\delta^2 = 26$  
  
![[../../../Extra Files/Pasted image 20250123103404.png|Pasted image 20250123103404.png]]  
$\frac{50}{-1+7i} \rightarrow \frac{50(-1-7i)}{(-1+7i)(-1-7i)} = \frac{-50-350i}{50} = -1-7i$  
$(\sum r_1,r_2) + \frac{5}{2}= r_3$  
$r_3 = -2+\frac{5}{2} = 0.5$  
$-1+7i+-1-7i+\frac{1}{2} = \frac{-b}{a}=\frac{-p}{2} = \frac{-3}{2} \qquad \therefore p=-3$  
$(-1+7i)(-1-7i)+\frac{1}{2}(-1+7i)+\frac{1}{2}(-1-7i)=\frac{q}{2}$  
$50-\frac{1}{2}+\frac{7i}{2}-\frac{1}{2} - \frac{7i}{2} = \frac{q}{2}$  
$49=\frac{q}{2} \qquad \therefore q=98$  
  
  
