---
tags:
  - Maths
  - Pure
date: 2025-01-22
---
---  
# Questions  
3. $3x^2 + kx - 4 = 0 \qquad x^2 + \frac{k}{3}x - \frac{4}{3} = 0$  
$(x - \alpha)(x - \beta)=0$  
$x^2 - \alpha{x} - \beta{x} + \alpha \beta$  
	a. $\alpha + \beta = -\frac{k}{3}$  
	b. $(\alpha+1)(\beta+1) = (\alpha \beta)+(\alpha + \beta)+1=\frac{4}{3} - \frac{k}{3} +1 = \frac{4+k}{3}+1 = \frac{7+k}{3} = \frac{1}{3}k$  
	c. $\alpha ^2 + \beta ^2 = (\alpha + \beta)^2 + 2\alpha \beta = (-\frac{k}{3})^2 + 2(\frac{4}{3}) = \frac{k^2}{9}+\frac{8}{3}$  
	